Generalize term syntax over constructor/variable identifiers

src/Utils/Utils.v
@@ -34,6 +34,13 @@ Ltac break :=
          | [H: exists x, _|-_]=> destruct H
          end.
 
+
+Ltac my_case eqnname exp :=
+  let casevar := fresh "casevar" in
+  remember exp as casevar eqn:eqnname;
+  destruct casevar; symmetry in eqnname.
+
+
 (* Performs inversion on H exactly when 
     either: 
     - no constructors can produce H and the goal is solved
@@ -63,6 +70,12 @@ Ltac solve_invert_constr_eq_lemma :=
 
 Ltac generic_crush rewrite_tac hint_auto :=
   repeat (intuition break; subst; rewrite_tac;
+          intuition unshelve hint_auto).
+(* Uses firstorder, which can have strange edge cases
+   and interacts poorly with terms
+ *)
+Ltac generic_firstorder_crush rewrite_tac hint_auto :=
+  repeat (intuition break; subst; rewrite_tac;
           firstorder unshelve hint_auto).
 (*try (solve [ repeat (unshelve f_equal; hint_auto)])). *)
 
@@ -88,22 +101,16 @@ fix all2 (s : list S) (t : list T) {struct s} : bool :=
   end.
 
 
+Ltac basic_utils_crush := let x := autorewrite with utils in * in
+                                  let y := eauto with utils in
+                                          generic_crush x y.
+Ltac basic_utils_firstorder_crush :=
+  let x := autorewrite with utils in * in
+          let y := eauto with utils in
+                  generic_firstorder_crush x y.
 
-Definition named_list_set (A : Set) :=list (string * A).
-Definition named_list (A : Type) :=list (string * A).
+Ltac basic_goal_prep := intros; break; simpl in *.
 
-Fixpoint named_list_lookup {A} default (l : named_list A) (s : string) : A :=
-  match l with
-  | [] => default
-  | (s', v)::l' =>
-    if eqb s s' then v else named_list_lookup default l' s
-  end.
-
-Lemma eqb_eq' n m : true = (n =? m) <-> n = m.
-Proof.
-  rewrite <- eqb_eq; intuition.
-Qed.
-Hint Rewrite eqb_eq' : utils.
 
 #[export] Hint Resolve in_nil : utils.
 #[export] Hint Resolve in_eq : utils.
@@ -114,105 +121,6 @@ Inductive len_eq {A} {B} : list A -> list B -> Type :=
 | len_eq_cons : forall a a' l l',
     len_eq l l' -> len_eq (a::l) (a'::l').
 
-Definition pair_map_snd {A B C} (f : B -> C) (p : A * B) :=
-  let (a,b) := p in (a, f b).
-Arguments pair_map_snd {A B C} f !p/.
-
-Definition named_map {A B} (f : A -> B) : named_list A -> named_list B
-  := map (pair_map_snd f).
-Arguments named_map {A B} f !l/.
-
-Definition fresh {A} n (nl : named_list A) : Prop :=
-  ~ List.In n (map fst nl).
-Arguments fresh : simpl never.
-
-(* These two lemmas should totally define fresh *)
-Lemma fresh_cons A n m (e:A) es : fresh n ((m,e)::es) <-> ~ n = m /\ fresh n es.
-Proof.
-  unfold fresh.
-  firstorder eauto.
-Qed.
-Hint Rewrite fresh_cons : utils.
-
-Lemma fresh_nil A n : fresh n (@nil (_*A)%type) <-> True.
-Proof.
-  unfold fresh; firstorder eauto.
-Qed.
-
-(*
-Lemma fresh_tail {A} n (l1 l2 : named_list A)
-  : fresh n (l1 ++ l2) -> fresh n l2.
-Proof using .
-  elim: l1; simpl; auto.
-  intros a l.
-  unfold fresh; simpl; intro IH.
-  rewrite !in_cons.
-  move /norP => [_] //.
-Qed.
-
-Lemma fresh_neq_in {A : eqType} n l n' (t : A)
-  : fresh n l -> (n',t) \in l -> ~~ (n'==n).
-Proof using .
-  elim: l; unfold fresh; simpl.
-  by cbv.
-  move => [n1 t1] l IH.
-  rewrite !in_cons.
-  move /norP => //= [nn1 nnl].
-  move /orP; case; eauto.
-  {
-    move /eqP.
-    case.
-    move -> => _.
-    
-    apply /negP.
-    move /eqP.
-    move: nn1=> /eqP.
-    intros nnneq nneq.
-    apply nnneq.
-    by symmetry.
-  }
-Qed.
-
-Lemma fresh_neq_in_fst {A : eqType} n (l : named_list A) n'
-  : fresh n l -> n' \in (map fst l) -> ~~ (n'==n).
-Proof using .
-  elim: l; unfold fresh; simpl.
-  by cbv.
-  move => [n1 t1] l IH.
-  rewrite !in_cons.
-  move /norP => //= [nn1 nnl].
-  move /orP; case; eauto.
-  {
-    move /eqP.
-    case.
-    move ->.
-    
-    apply /negP.
-    move /eqP.
-    move: nn1=> /eqP.
-    intros nnneq nneq.
-    apply nnneq.
-    by symmetry.
-  }
-Qed.
- *)
-
-(*
-Fixpoint all_notin (l : list string) : Prop :=
-  match l with
-  | [] => True
-  | n::l' => (~ List.In n l') /\ all_notin l'
-  end.
-*)
-
-Fixpoint all_fresh {A} (l : named_list A) :=
-  match l with
-  | [] => True
-  | (n,_)::l' => fresh n l' /\ all_fresh l'
-  end.
-Arguments all_fresh {_} !_ /.
-
-
 Hint Rewrite pair_equal_spec : utils.
 
 Lemma pair_fst_in {N A} l (n: N) (a : A)
@@ -222,82 +130,6 @@ Proof using.
 Qed.
 #[export] Hint Resolve pair_fst_in : utils.
 
-Lemma named_map_fst_eq {A B} (f : A -> B) l
-  : map fst (named_map f l) = map fst l.
-Proof using .
-  induction l; intros; break; simpl in *; f_equal; eauto.
-Qed.
-
-(*
-Lemma in_map_snd {A B : eqType} e (l : list (A*B))
-  : e \in (map snd l) -> exists n, (n,e) \in l.
-Proof using .
-  elim: l; simpl; [ by inversion|];
-    intros; break; simpl in *.
-  move: H0; rewrite in_cons; move /orP; case.
-  {
-    move => /eqP ->.
-    exists s.
-    rewrite in_cons.
-    apply /orP; left; apply eq_refl.
-  }
-  {
-    move /H.
-    case.
-    intros.
-    exists x.
-    rewrite in_cons; apply /orP; right; done.
-  }
-Qed.
-*)
-
-
-(*Moved out of the module because Coq seems
-  to include them at the the top level anyway
- *)
-Declare Custom Entry monadic_do.
-
-Module OptionMonad.
-  (* TODO: use general monad instead of duplicating*)
-  
-  Notation "'do' e" := (e) (at level 92, e custom monadic_do).
-
-  Notation "p <- e ; b" :=
-    (match e with
-     | Some (p) => b
-     | _ => None
-     end)
-      (in custom monadic_do at level 90, left associativity, p pattern at level 0, e constr, b custom monadic_do).
-
-  Notation "'ret' e" := (Some e) (in custom monadic_do at level 90, e constr).
-  
-  Notation "'let' p := e ; b" :=
-    (let p := e in b)
-      (in custom monadic_do at level 90, left associativity, p pattern at level 0, e constr, b custom monadic_do).
-
-  Notation "! e ; b" :=
-    (if e then b else None)
-      (in custom monadic_do at level 90, left associativity, e constr, b custom monadic_do).
-
-  Section Mmap.
-    Context  {A B} (f : A -> option B).
-    Fixpoint Mmap (l_a : list A) : option (list B) :=
-      match l_a with
-      | [] => do ret []
-               | a::l_a' =>
-                 do l_b' <- Mmap l_a';
-                 b <- f a;
-              ret (b::l_b')
-      end.
-  End Mmap.
-End OptionMonad.
-
-
-Fixpoint named_list_lookup_err {A} (l : named_list A) s : option A :=
-  match l with
-  | [] => None
-  | (s', v) :: l' => if (s =? s')%string then Some v else named_list_lookup_err l' s
-  end.
 
 Ltac case_match :=match goal with
   | [|- context[match ?e with _ => _ end]]
@@ -360,27 +192,94 @@ Proof.
 Qed.
 Hint Rewrite invert_eq_cons_cons : utils.
 
-Ltac my_case eqnname exp :=
-  let casevar := fresh "casevar" in
-  remember exp as casevar eqn:eqnname;
-  destruct casevar; symmetry in eqnname.
+(*TODO: does this exist somewhere I can use?
+  TODO: include minimum necessary to prove the given properties
+*)
+Class Eqb (A : Type) :=
+  {
+  eqb : A -> A -> bool;
+  eqb_eq : forall n m : A, eqb n m = true <-> n = m;
+  eqb_neq : forall x y : A, (eqb x y) = false <-> x <> y;
+  eqb_refl : forall x : A, (eqb x x) = true;
+  Eqb_dec : forall (s1 s2 : A), {s1 = s2} + {s1 <> s2}
+  }.
+#[export] Hint Rewrite @eqb_eq : utils.
+#[export] Hint Rewrite @eqb_neq : utils.
+#[export] Hint Rewrite @eqb_refl : utils.
 
-Hint Rewrite eqb_eq : utils.
-Hint Rewrite eqb_neq : utils.
-Hint Rewrite eqb_refl : utils.
+(* Not defined as a record so that firstorder doesn't mess with it*)
+Definition WithDefault (A : Type) := A.
+Definition default {A} {d : WithDefault A} := d.
+Existing Class WithDefault.
 
-Ltac basic_utils_crush := let x := autorewrite with utils in * in
-                                  let y := eauto with utils in
-                                          generic_crush x y.
+(* TODO: separate file? *)
+Section NamedList.
+  Context {S : Type}
+          `{Eqb S}.
 
-Ltac basic_goal_prep := intros; break; simpl in *.
+Definition named_list (A : Type) :=list (S * A).
+
+Fixpoint named_list_lookup {A} default (l : named_list A) (s : S) : A :=
+  match l with
+  | [] => default
+  | (s', v)::l' =>
+    if eqb s s' then v else named_list_lookup default l' s
+  end.
+
+
+
+Definition pair_map_snd {A B C} (f : B -> C) (p : A * B) :=
+  let (a,b) := p in (a, f b).
+Arguments pair_map_snd {A B C} f !p/.
+
+Definition named_map {A B} (f : A -> B) : named_list A -> named_list B
+  := map (pair_map_snd f).
+Arguments named_map {A B} f !l/.
+
+Definition fresh {A} n (nl : named_list A) : Prop :=
+  ~ List.In n (map fst nl).
+Arguments fresh : simpl never.
+
+(* These two lemmas should totally define fresh *)
+Lemma fresh_cons A n m (e:A) es : fresh n ((m,e)::es) <-> ~ n = m /\ fresh n es.
+Proof.
+  unfold fresh.
+  firstorder eauto.
+Qed.
+
+Lemma fresh_nil A n : fresh n (@nil (_*A)%type) <-> True.
+Proof.
+  unfold fresh; firstorder eauto.
+Qed.
+
+Fixpoint all_fresh {A} (l : named_list A) :=
+  match l with
+  | [] => True
+  | (n,_)::l' => fresh n l' /\ all_fresh l'
+  end.
+Arguments all_fresh {_} !_ /.
+
+
+Lemma named_map_fst_eq {A B} (f : A -> B) l
+  : map fst (named_map f l) = map fst l.
+Proof using .
+  induction l; intros; break; simpl in *; f_equal; eauto.
+Qed.
+
+
+Fixpoint named_list_lookup_err {A} (l : named_list A) s : option A :=
+  match l with
+  | [] => None
+  | (s', v) :: l' => if eqb s s' then Some v else named_list_lookup_err l' s
+  end.
+
 
 Lemma named_list_lookup_err_in {A} c n (t : A)
   : Some t = named_list_lookup_err c n -> In (n,t) c.
 Proof using .
   induction c; basic_goal_prep.
   basic_utils_crush.
-  my_case Heq (n =? s); basic_utils_crush.
+  my_case Heq (eqb n s); basic_utils_crush.
 Qed.
 
 Lemma all_fresh_named_list_lookup_err_in A c n (t : A)
@@ -388,20 +287,15 @@ Lemma all_fresh_named_list_lookup_err_in A c n (t : A)
 Proof using .
   induction c; basic_goal_prep.
   basic_utils_crush.
-  my_case Heq (n =? s); basic_utils_crush.  
+  my_case Heq (eqb n s); basic_utils_crush.  
 Qed.
-(*Note: this is a bit dangerous since the list might not be all-fresh,
-  but in this project all lists should be
-*)
-Hint Rewrite all_fresh_named_list_lookup_err_in : utils.
 
 Lemma fresh_named_map A B l (f : A -> B) n
   : fresh n (named_map f l) <-> fresh n l.
 Proof.
   induction l; basic_goal_prep;
-    basic_utils_crush.
+    basic_utils_firstorder_crush.
 Qed.
-Hint Rewrite fresh_named_map : utils.
 
 Fixpoint with_names_from {A B} (c : named_list A) (l : list B) : named_list B :=
   match c, l with
@@ -417,7 +311,216 @@ Lemma map_fst_with_names_from A B (c : named_list A) (l : list B)
 Proof.
   revert l; induction c; destruct l; basic_goal_prep; basic_utils_crush.
 Qed.
-Hint Rewrite map_fst_with_names_from : utils.
+
+
+Lemma named_list_lookup_none {A} l s (a:A)
+  : None = named_list_lookup_err l s ->
+    ~ In (s, a) l.
+Proof.
+  induction l; basic_goal_prep; basic_utils_crush.
+  my_case Hs (eqb s s0); basic_goal_prep; basic_utils_crush.
+Qed.
+
+
+Lemma in_named_map A B (f : A -> B) l n x
+  : In (n,x) l -> In (n, f x) (named_map f l).
+Proof.
+  induction l; basic_goal_prep; basic_utils_crush.
+Qed.
+
+
+Lemma in_all_fresh_same {A} (a b : A) l s
+  : all_fresh l -> In (s,a) l -> In (s,b) l -> a = b.
+Proof.  
+  induction l; basic_goal_prep; basic_utils_crush.
+Qed.
+
+(* decomposes the way you want \in to on all_fresh lists*)
+Fixpoint in_once {A} n e (l : named_list A) : Prop :=
+  match l with
+  | [] => False
+  | (n',e')::l' =>
+    ((n = n') /\ (e = e')) \/ ((~n = n') /\ (in_once n e l'))
+  end.
+
+Arguments in_once {A} n e !l/.
+
+Lemma in_once_notin {A} n (e : A) l
+  : ~ In n (map fst l) -> ~(in_once n e l).
+Proof using .
+  induction l; basic_goal_prep;
+  basic_utils_crush.
+Qed.
+
+Lemma all_fresh_in_once {A} n (e : A) l
+  : all_fresh l -> (In (n,e) l) <-> in_once n e l.
+Proof.
+  induction l; basic_goal_prep; basic_utils_crush.
+Qed.  
+
+
+
+Lemma with_names_from_map_is_named_map A B C (f : A -> B) (l1 : named_list C) l2
+  : with_names_from l1 (map f l2) = named_map f (with_names_from l1 l2).
+Proof.
+  revert l2; induction l1;
+    destruct l2; break; subst; simpl; f_equal; eauto.
+Qed.
+(* TODO: do I want to rewrite like this?
+  Hint Rewrite with_names_from_map_is_named_map : utils.*)
+
+Lemma combine_map_fst_is_with_names_from A B (c : named_list A) (s : list B)
+  : combine (map fst c) s = with_names_from c s.
+Proof.
+  revert s; induction c; destruct s;
+    basic_goal_prep;
+    basic_utils_crush.
+Qed.
+
+Lemma named_map_length A B (f : A -> B) l
+  : length (named_map f l) = length l.
+Proof.
+  induction l; basic_goal_prep; basic_utils_crush.
+Qed.
+
+
+Lemma fresh_notin A n (a:A) l
+  : fresh n l -> ~In (n,a) l.
+Proof.
+  unfold fresh.
+  intuition eauto using pair_fst_in.
+Qed.
+
+
+Definition fresh_dec {A} x (l : named_list A) : {fresh x l} + {~ fresh x l}.
+  refine(if in_dec Eqb_dec x (map fst l) then right _ else left _);
+    basic_utils_crush.
+Defined.
+
+Definition compute_fresh {A} x (l : named_list A)  :=
+  if fresh_dec x l then true else false.
+
+Lemma use_compute_fresh {A} x (l : named_list A) 
+  : compute_fresh x l = true -> fresh x l.
+Proof.
+  unfold compute_fresh.
+  destruct (fresh_dec x l); easy.
+Qed.
+
+
+Lemma fresh_app A s (l1 l2 : named_list A)
+  : fresh s (l1 ++ l2) <-> fresh s l1 /\ fresh s l2.
+Proof.
+  induction l1; basic_goal_prep; basic_utils_firstorder_crush.
+Qed.
+
+
+#[local] Hint Resolve fresh_notin : utils.
+#[local] Hint Rewrite fresh_app : utils.
+#[local] Hint Rewrite in_app_iff : utils.
+Lemma all_fresh_insert_is_fresh A (a:A) l1 l2 s
+  : all_fresh (l1++(s,a)::l2) ->
+    fresh s l1.
+Proof.
+  induction l1; basic_goal_prep;
+  basic_utils_firstorder_crush.  
+Qed.
+Local Hint Resolve all_fresh_insert_is_fresh : utils.
+
+Lemma all_fresh_insert_rest_is_fresh A (a:A) l1 l2 s
+  : all_fresh (l1++(s,a)::l2) ->
+    all_fresh (l1++l2).
+Proof.
+  induction l1; basic_goal_prep; basic_utils_firstorder_crush.
+Qed.
+
+
+Fixpoint compute_all_fresh {A} (l : named_list A) : bool :=
+  match l with
+  | [] => true
+  | (x,_)::l' => (compute_fresh x l') && (compute_all_fresh l')
+  end.
+#[local] Hint Rewrite Bool.andb_true_iff : utils.
+
+Lemma use_compute_all_fresh A (l : named_list A)
+  : compute_all_fresh l = true -> all_fresh l.
+Proof.
+  induction l; basic_goal_prep; basic_utils_crush.
+  apply use_compute_fresh; eauto.
+Qed.
+
+
+(* TODO: shouldn't be needed if I flip order equations reliably
+   TODO: should be in a different location
+*)
+Lemma eqb_eq' n m : true = (eqb n m) <-> n = m.
+Proof.
+  rewrite <- eqb_eq; intuition.
+Qed.
+
+End NamedList.
+
+#[export] Hint Rewrite @fresh_cons : utils.
+#[export] Hint Rewrite @fresh_named_map : utils.
+#[export] Hint Rewrite @map_fst_with_names_from : utils.
+(*Note: this is a bit dangerous since the list might not be all-fresh,
+  but in this project all lists should be
+*)
+#[export] Hint Rewrite @all_fresh_named_list_lookup_err_in : utils.
+#[export] Hint Resolve @named_list_lookup_none : utils.
+#[export] Hint Resolve @in_named_map : utils.
+#[export] Hint Rewrite @combine_map_fst_is_with_names_from : utils.
+#[export] Hint Rewrite @named_map_length : utils.
+#[export] Hint Rewrite map_length : utils.
+#[export] Hint Resolve @fresh_notin : utils.
+#[export] Hint Rewrite @fresh_app : utils.
+#[export] Hint Rewrite in_app_iff : utils.
+#[export] Hint Resolve @all_fresh_insert_rest_is_fresh : utils.
+#[export] Hint Rewrite Bool.andb_true_iff : utils.
+#[export] Hint Rewrite @eqb_eq' : utils.
+
+
+(*Moved out of the module because Coq seems
+  to include them at the the top level anyway
+ *)
+Declare Custom Entry monadic_do.
+
+Module OptionMonad.
+  (* TODO: use general monad instead of duplicating*)
+  
+  Notation "'do' e" := (e) (at level 92, e custom monadic_do).
+
+  Notation "p <- e ; b" :=
+    (match e with
+     | Some (p) => b
+     | _ => None
+     end)
+      (in custom monadic_do at level 90, left associativity, p pattern at level 0, e constr, b custom monadic_do).
+
+  Notation "'ret' e" := (Some e) (in custom monadic_do at level 90, e constr).
+  
+  Notation "'let' p := e ; b" :=
+    (let p := e in b)
+      (in custom monadic_do at level 90, left associativity, p pattern at level 0, e constr, b custom monadic_do).
+
+  Notation "! e ; b" :=
+    (if e then b else None)
+      (in custom monadic_do at level 90, left associativity, e constr, b custom monadic_do).
+
+  Section Mmap.
+    Context  {A B} (f : A -> option B).
+    Fixpoint Mmap (l_a : list A) : option (list B) :=
+      match l_a with
+      | [] => do ret []
+               | a::l_a' =>
+                 do l_b' <- Mmap l_a';
+                 b <- f a;
+              ret (b::l_b')
+      end.
+  End Mmap.
+End OptionMonad.
+
+
 
 
 Fixpoint sublist {A} (s l : list A) : Prop :=
@@ -458,6 +561,7 @@ Proof.
 Qed.
 #[export] Hint Resolve sublist_l_cons_l : utils.
 
+(*TODO: redefine as skipn?*)
 (* Reduce size of language terms for smaller goals *)
 Fixpoint nth_tail {A} (n: nat) (l : list A) : list A :=
   match n,l with
@@ -480,56 +584,6 @@ Proof.
 Qed.
 Hint Rewrite nth_tail_S_cons : utils.
 
-(*
-Lemma nth_tail_cons_eq {A} (a:A) l n l'
-  : a::l = nth_tail n l' -> l = nth_tail n.+1 l'.
-Proof.
-  revert a l l'.
-  induction n.
-  {
-    intros; destruct l';
-      cbv[nth_tail] in*;
-      inversion H; auto.
-  }
-  {
-    intros; destruct l'.
-    {
-      cbv[nth_tail] in*;
-        inversion H; auto.
-    }
-    {
-      rewrite nth_tail_S_cons.
-      rewrite nth_tail_S_cons in H.
-      eauto.
-    }
-  }
-Qed.
-*)
-
-(*
-Lemma nth_tail_0 {A} (l : list A) : nth_tail 0 l = l.
-Proof. reflexivity. Qed.
-
-      
-Lemma nth_tail_show_hd {A} (default:A) n l
-  : size l > n ->
-    nth_tail n l = (nth default l n) ::(nth_tail (S n) l).
-Proof.
-  elim: n l; intros.
-  {
-    destruct l; simpl in *; inversion H.
-    rewrite nth_tail_S_cons.
-    rewrite !nth_tail_0.
-    reflexivity.
-  }   
-  {
-    destruct l; simpl in *; inversion H0.
-    clear H2.
-    rewrite !nth_tail_S_cons.
-    apply H; exact H0.
-  }
-Qed.    
-*)
 
 (*redefined to use the right concatenation*)
 Definition flat_map {A B} (f : A -> list B) :=
@@ -538,127 +592,6 @@ Definition flat_map {A B} (f : A -> list B) :=
   | [] => []
   | x :: t => (f x ++ flat_map t)
   end.
-
-(*
-Lemma included_flatmap {A B:eqType} l1 l2 (f : A -> list B)
-    : (forall x, x \in l1 -> included (f x) l2)->
-      included (flat_map f l1) l2.
-Proof.  
-  induction l1; simpl; auto.
-  intro fall.
-  rewrite included_app; eauto.
-  apply /andP; split.
-  apply fall; apply mem_head.
-  apply IHl1; intros.
-  apply fall.
-  rewrite in_cons.
-  apply /orP; right; auto.
-Qed.
-*)
-
-Lemma in_all_fresh_same {A} (a b : A) l s
-  : all_fresh l -> In (s,a) l -> In (s,b) l -> a = b.
-Proof.  
-  induction l; basic_goal_prep; basic_utils_crush.
-Qed.
-
-(*
-Lemma named_list_lookup_err_none {A} (l : named_list A) n
-  : n \notin (map fst l) ->
-    named_list_lookup_err l n = None.
-Proof.
-  elim: l; simpl; auto.
-  intros; break; simpl.
-  rewrite in_cons in H0.
-  move: H0 => /norP []; simpl; intros.
-  apply negbTE in a0;
-    change (n =? s = false)%string in a0;
-    rewrite a0.
-  auto.
-Qed.
-
-
-  
-Lemma named_list_lookup_err_inb {A : eqType} l x (v:A)
-  : all_fresh l ->
-    named_list_lookup_err l x == Some v = ((x,v) \in l).
-Proof.
-  induction l; break; [by compute | simpl]; intros; break.
-  case_match.
-  {
-    match goal with
-      [H : true = (?a =? ?b)%string |-_]=>
-      symmetry in H; change (is_true (a == b)) in H;
-        move: H => /eqP H; subst
-    end.
-    case veqs0: (s0 == v).
-    {
-      move:veqs0 => /eqP veqs0; subst.
-      rewrite in_cons.
-      rewrite !eq_refl.
-      by compute.
-    }
-    {
-      rewrite in_cons.
-      cbn.
-      rewrite veqs0 eqb_refl.
-      rewrite eq_sym in veqs0.
-      rewrite veqs0.
-      simpl.
-      simpl in IHl.
-      rewrite <- IHl; auto.
-      rewrite named_list_lookup_err_none; auto.
-    }
-  }
-  {
-      rewrite in_cons.
-      cbn.
-      rewrite <- HeqH1.
-      cbn.
-      auto.
-  }
-Qed.
-*)
-
-Lemma named_list_lookup_none {A} l s (a:A)
-  : None = named_list_lookup_err l s ->
-    ~ In (s, a) l.
-Proof.
-  induction l; basic_goal_prep; basic_utils_crush.
-  my_case Hs (s=? s0); basic_goal_prep; basic_utils_crush.
-Qed.
-#[export] Hint Resolve named_list_lookup_none : utils.
-
-
-Lemma in_named_map A B (f : A -> B) l n x
-  : In (n,x) l -> In (n, f x) (named_map f l).
-Proof.
-  induction l; basic_goal_prep; basic_utils_crush.
-Qed.
-#[export] Hint Resolve in_named_map : utils.
-
-(* decomposes the way you want \in to on all_fresh lists*)
-Fixpoint in_once {A} n e (l : named_list A) : Prop :=
-  match l with
-  | [] => False
-  | (n',e')::l' =>
-    ((n = n') /\ (e = e')) \/ ((~n = n') /\ (in_once n e l'))
-  end.
-
-Arguments in_once {A} n e !l/.
-
-Lemma in_once_notin {A} n (e : A) l
-  : ~ In n (map fst l) -> ~(in_once n e l).
-Proof using .
-  induction l; basic_goal_prep;
-  basic_utils_crush.
-Qed.
-
-Lemma all_fresh_in_once {A} n (e : A) l
-  : all_fresh l -> (In (n,e) l) <-> in_once n e l.
-Proof using .
-  induction l; basic_goal_prep; basic_utils_crush.
-Qed.  
 
 Section All.
   Context {A} (P : A -> Prop).
@@ -679,57 +612,6 @@ Qed.
 
 Hint Rewrite pair_equal_spec : utils.
 
-
-
-Lemma with_names_from_map_is_named_map A B C (f : A -> B) (l1 : named_list C) l2
-  : with_names_from l1 (map f l2) = named_map f (with_names_from l1 l2).
-Proof.
-  revert l2; induction l1;
-    destruct l2; break; subst; simpl; f_equal; eauto.
-Qed.
-(* TODO: do I want to rewrite like this?
-  Hint Rewrite with_names_from_map_is_named_map : utils.*)
-
-Lemma combine_map_fst_is_with_names_from A B (c : named_list A) (s : list B)
-  : combine (map fst c) s = with_names_from c s.
-Proof.
-  revert s; induction c; destruct s;
-    basic_goal_prep;
-    basic_utils_crush.
-Qed.
-Hint Rewrite combine_map_fst_is_with_names_from : utils.
-
-Lemma named_map_length A B (f : A -> B) l
-  : length (named_map f l) = length l.
-Proof.
-  induction l; basic_goal_prep; basic_utils_crush.
-Qed.
-Hint Rewrite named_map_length : utils.
-Hint Rewrite map_length : utils.
-
-
-Lemma fresh_notin A n (a:A) l
-  : fresh n l -> ~In (n,a) l.
-Proof.
-  unfold fresh.
-  intuition eauto using pair_fst_in.
-Qed.
-#[export] Hint Resolve fresh_notin : utils.
-
-
-Definition fresh_dec {A} x (l : named_list A) : {fresh x l} + {~ fresh x l}.
-  refine(if in_dec string_dec x (map fst l) then right _ else left _);
-    basic_utils_crush.
-Defined.
-
-Definition compute_fresh {A} x (l : named_list A)  := if fresh_dec x l then true else false.
-
-Lemma use_compute_fresh {A} x (l : named_list A) 
-  : compute_fresh x l = true -> fresh x l.
-Proof.
-  unfold compute_fresh.
-  destruct (fresh_dec x l); easy.
-Qed.
 
 
 Lemma sublist_nil A (l : list A) : sublist [] l.
@@ -757,33 +639,6 @@ Proof.
   intros; unfold nth_tail; reflexivity.
 Qed.
 
-Lemma fresh_app A s (l1 l2 : named_list A)
-  : fresh s (l1 ++ l2) <-> fresh s l1 /\ fresh s l2.
-Proof.
-  induction l1; basic_goal_prep; basic_utils_crush.
-Qed.
-Hint Rewrite fresh_app : utils.
-Hint Rewrite in_app_iff : utils.
-
-
-Lemma all_fresh_insert_is_fresh A (a:A) l1 l2 s
-  : all_fresh (l1++(s,a)::l2) ->
-    fresh s l1.
-Proof.
-  induction l1; basic_goal_prep;
-  basic_utils_crush.  
-Qed.
-Local Hint Resolve all_fresh_insert_is_fresh : utils.
-
-Lemma all_fresh_insert_rest_is_fresh A (a:A) l1 l2 s
-  : all_fresh (l1++(s,a)::l2) ->
-    all_fresh (l1++l2).
-Proof.
-  induction l1; basic_goal_prep; basic_utils_crush.
-Qed.
-#[export] Hint Resolve all_fresh_insert_rest_is_fresh : utils.
-
-
 Definition set_eq {A} (l1 l2 : list A) :=
   incl l1 l2 /\ incl l2 l1.
 
@@ -803,20 +658,6 @@ Proof.
   split; intros; break; eauto using incl_cons, incl_cons_inv.
 Qed.
 Hint Rewrite incl_cons : utils.
-
-Fixpoint compute_all_fresh {A} (l : named_list A) : bool :=
-  match l with
-  | [] => true
-  | (x,_)::l' => (compute_fresh x l') && (compute_all_fresh l')
-  end.
-Hint Rewrite Bool.andb_true_iff : utils.
-
-Lemma use_compute_all_fresh A (l : named_list A)
-  : compute_all_fresh l = true -> all_fresh l.
-Proof.
-  induction l; basic_goal_prep; basic_utils_crush.
-  apply use_compute_fresh; eauto.
-Qed.
 
 Lemma nth_tail_to_cons A l n (x:A)
   : nth_error l n = Some x ->
@@ -877,5 +718,6 @@ Fixpoint incl_dec {A} (eq_dec : forall s1 s2 : A, {s1 = s2} + {s1 <> s2})
          | [] => left _
          | a::l1' =>
            SB! (in_dec eq_dec a l2) SB& (incl_dec _ _ l1' l2)
-         end); basic_utils_crush.
+         end); basic_utils_firstorder_crush.
 Defined.
+
