src/named/Rule.v
@@ -11,12 +11,26 @@ From Named Require Import Term.
 Import Term.Notations.
 Import SumboolNotations.
 
-Inductive rule : Set :=
-| sort_rule :  ctx -> list string (*explicit args*) -> rule
-| term_rule :  ctx -> list string (*explicit args*) -> sort -> rule
+
+Section WithVar.
+  Context (V : Type)
+          {V_Eqb : Eqb V}
+          {V_default : WithDefault V}.
+
+  Notation named_list := (@named_list V).
+  Notation named_map := (@named_map V).
+  Notation term := (@term V).
+  Notation ctx := (@ctx V).
+  Notation sort := (@sort V).
+
+Inductive rule :=
+| sort_rule :  ctx -> list V (*explicit args*) -> rule
+| term_rule :  ctx -> list V (*explicit args*) -> sort -> rule
 | sort_eq_rule : ctx -> sort -> sort -> rule
 | term_eq_rule : ctx -> term -> term -> sort -> rule.
-#[export] Hint Constructors rule : term.
+Hint Constructors rule : term.
+
+Instance default_rule : WithDefault rule := sort_rule [] [].
 
 Definition lang := named_list rule.
 
@@ -24,11 +38,12 @@ Lemma invert_eq_sort_rule_sort_rule c c' args args'
   : sort_rule c args = sort_rule c' args' <-> c = c' /\ args = args'.
 Proof. solve_invert_constr_eq_lemma. Qed.
 Hint Rewrite invert_eq_sort_rule_sort_rule : term.
-  
+
 Lemma invert_eq_sort_rule_term_rule c c' args args' t'
   : sort_rule c args = term_rule c' args' t' <-> False.
 Proof. solve_invert_constr_eq_lemma. Qed.
 Hint Rewrite invert_eq_sort_rule_term_rule : term.
+
 
 Lemma invert_eq_sort_rule_sort_eq_rule c c' args t1' t2'
   : sort_rule c args = sort_eq_rule c' t1' t2' <-> False.
@@ -59,7 +74,6 @@ Lemma invert_eq_term_rule_term_eq_rule c c' args t e1' e2' t'
   : term_rule c args t = term_eq_rule c' e1' e2' t' <-> False.
 Proof. solve_invert_constr_eq_lemma. Qed.
 Hint Rewrite invert_eq_term_rule_term_eq_rule : term.
-
 
 Lemma invert_eq_sort_eq_rule_sort_rule c c' args' t1 t2
   : sort_eq_rule c t1 t2 = sort_rule c' args' <-> False.
@@ -100,6 +114,101 @@ Lemma invert_eq_term_eq_rule_term_eq_rule c c' e1 e2 e1' e2' t t'
   : term_eq_rule c e1 e2 t = term_eq_rule c' e1' e2' t' <-> c = c' /\ e1 = e1' /\ e2 = e2' /\ t = t'.
 Proof. solve_invert_constr_eq_lemma. Qed.
 Hint Rewrite invert_eq_term_eq_rule_term_eq_rule : term.
+
+Notation well_scoped := (@well_scoped V V_Eqb).
+
+Definition ws_rule r : Prop :=
+  match r with
+  | sort_rule c args => sublist args (map fst c) /\ ws_ctx c
+  | term_rule c args t => sublist args (map fst c) /\ (ws_ctx c)
+                          /\ (well_scoped (map fst c) t)
+  | sort_eq_rule c t t'=>
+    (ws_ctx c) /\ (well_scoped (map fst c) t)
+    /\ (well_scoped (map fst c) t')
+  | term_eq_rule c e e' t =>
+    (ws_ctx c) /\ (well_scoped (map fst c) e)
+    /\ (well_scoped (map fst c) e') /\ (well_scoped (map fst c) t)
+  end.
+
+Definition ws_lang (l : lang) : Prop :=
+  (all_fresh l) /\ (all ws_rule (map snd l)).
+
+Arguments ws_lang !l/.
+
+Lemma rule_in_ws l n r : ws_lang l -> In (n,r) l -> ws_rule r.
+Proof using .
+  induction l; 
+    basic_goal_prep;
+    basic_term_firstorder_crush.
+Qed.
+
+Lemma reconstruct_ws_lang l
+  : all_fresh l /\ all ws_rule (map snd l) -> ws_lang l.
+Proof.
+  eauto.
+Qed.
+Hint Resolve reconstruct_ws_lang : term.
+
+Lemma ws_lang_all_ws_rule l
+  : ws_lang l -> all ws_rule (map snd l).
+Proof.
+  unfold ws_lang; intuition.
+Qed.
+Hint Resolve ws_lang_all_ws_rule : term.
+
+
+Definition rule_eq_dec (r1 r2 : rule) : {r1 = r2} + {~ r1 = r2}.
+  refine(match r1, r2 with
+         | sort_rule c args, sort_rule c' args' =>
+           SB! (ctx_eq_dec c c') SB& (list_eq_dec Eqb_dec args args')
+         | term_rule c args t, term_rule c' args' t' =>
+           SB! (ctx_eq_dec c c') SB&
+           (list_eq_dec Eqb_dec args args') SB&
+           (sort_eq_dec t t')
+         | sort_eq_rule c t1 t2, sort_eq_rule c' t1' t2' =>
+           SB! (ctx_eq_dec c c') SB&
+           (sort_eq_dec t1 t1') SB&
+           (sort_eq_dec t2 t2')
+         | term_eq_rule c e1 e2 t, term_eq_rule c' e1' e2' t' =>
+           SB! (ctx_eq_dec c c') SB&
+           (term_eq_dec e1 e1') SB&
+           (term_eq_dec e2 e2') SB&
+           (sort_eq_dec t t')
+         | _,_ => _
+         end); basic_term_crush.
+Defined.
+
+Definition compute_incl_lang (l1 l2 : lang) :=
+  if incl_dec (pair_eq_dec Eqb_dec rule_eq_dec) l1 l2 then true else false.
+
+Lemma use_compute_incl_lang (l1 l2 : lang)
+  : compute_incl_lang l1 l2 = true -> incl l1 l2.
+Proof.
+  unfold compute_incl_lang.
+  destruct (incl_dec _ l1 l2); easy.
+Qed.
+
+
+End WithVar.
+#[export] Hint Constructors rule : term.
+#[export] Hint Rewrite invert_eq_sort_rule_sort_rule : term.
+#[export] Hint Rewrite invert_eq_sort_rule_term_rule : term.
+#[export] Hint Rewrite invert_eq_sort_rule_sort_eq_rule : term.
+#[export] Hint Rewrite invert_eq_sort_rule_term_eq_rule : term.
+#[export] Hint Rewrite invert_eq_term_rule_sort_rule : term.
+#[export] Hint Rewrite invert_eq_term_rule_term_rule : term.
+#[export] Hint Rewrite invert_eq_term_rule_sort_eq_rule : term.
+#[export] Hint Rewrite invert_eq_term_rule_term_eq_rule : term.
+#[export] Hint Rewrite invert_eq_sort_eq_rule_sort_rule : term.
+#[export] Hint Rewrite invert_eq_sort_eq_rule_term_rule : term.
+#[export] Hint Rewrite invert_eq_sort_eq_rule_sort_eq_rule : term.
+#[export] Hint Rewrite invert_eq_sort_eq_rule_term_eq_rule : term.
+#[export] Hint Rewrite invert_eq_term_eq_rule_sort_rule : term.
+#[export] Hint Rewrite invert_eq_term_eq_rule_term_rule : term.
+#[export] Hint Rewrite invert_eq_term_eq_rule_sort_eq_rule : term.
+#[export] Hint Rewrite invert_eq_term_eq_rule_term_eq_rule : term.
+#[export] Hint Resolve reconstruct_ws_lang : term.
+#[export] Hint Resolve ws_lang_all_ws_rule : term.
 
 
 (*Moved out of the module because Coq seems
@@ -231,95 +340,3 @@ Check [:= "G" : #"env", "A" : #"ty" "G", "B" : #"ty" "G",
       ]%rule.
 
 End Notations.
-
-(*
-(*
-Definition ws_rule (r : rule) : bool :=
-  match r with
-  | {| c |- sort} => ws_ctx c
-  | {| c |- t} => ws_ctx c && ws_term (size c) t
-  | {< c |- s1 <# s2} =>
-    ws_ctx c
-           && ws_term (size c) s1
-           && ws_term (size c) s2
-  | {< c |- e1 <# e2 .: s} =>
-    ws_ctx c
-           && ws_term (size c) e1
-           && ws_term (size c) e2
-           && ws_term (size c) s
-  end.
-
-Definition ws_lang : lang -> bool := List.forallb ws_rule.
-*)
-*)
-
-
-Definition ws_rule r : Prop :=
-  match r with
-  | sort_rule c args => sublist args (map fst c) /\ ws_ctx c
-  | term_rule c args t => sublist args (map fst c) /\ (ws_ctx c) /\ (well_scoped (map fst c) t)
-  | sort_eq_rule c t t'=>
-    (ws_ctx c) /\ (well_scoped (map fst c) t)
-    /\ (well_scoped (map fst c) t')
-  | term_eq_rule c e e' t =>
-    (ws_ctx c) /\ (well_scoped (map fst c) e)
-    /\ (well_scoped (map fst c) e') /\ (well_scoped (map fst c) t)
-  end.
-
-Definition ws_lang (l : lang) : Prop :=
-  (all_fresh l) /\ (all ws_rule (map snd l)).
-
-Arguments ws_lang !l/.
-
-Lemma rule_in_ws l n r : ws_lang l -> In (n,r) l -> ws_rule r.
-Proof using .
-  induction l; 
-    basic_goal_prep;
-    basic_term_crush.
-Qed.
-
-Lemma reconstruct_ws_lang l
-  : all_fresh l /\ all ws_rule (map snd l) -> ws_lang l.
-Proof.
-  eauto.
-Qed.
-#[export] Hint Resolve reconstruct_ws_lang : term.
-
-Lemma ws_lang_all_ws_rule l
-  : ws_lang l -> all ws_rule (map snd l).
-Proof.
-  unfold ws_lang; intuition.
-Qed.
-#[export] Hint Resolve ws_lang_all_ws_rule : term.
-
-
-Definition rule_eq_dec (r1 r2 : rule) : {r1 = r2} + {~ r1 = r2}.
-  refine(match r1, r2 with
-         | sort_rule c args, sort_rule c' args' =>
-           SB! (ctx_eq_dec c c') SB& (list_eq_dec string_dec args args')
-         | term_rule c args t, term_rule c' args' t' =>
-           SB! (ctx_eq_dec c c') SB&
-           (list_eq_dec string_dec args args') SB&
-           (sort_eq_dec t t')
-         | sort_eq_rule c t1 t2, sort_eq_rule c' t1' t2' =>
-           SB! (ctx_eq_dec c c') SB&
-           (sort_eq_dec t1 t1') SB&
-           (sort_eq_dec t2 t2')
-         | term_eq_rule c e1 e2 t, term_eq_rule c' e1' e2' t' =>
-           SB! (ctx_eq_dec c c') SB&
-           (term_eq_dec e1 e1') SB&
-           (term_eq_dec e2 e2') SB&
-           (sort_eq_dec t t')
-         | _,_ => _
-         end); basic_term_crush.
-Defined.
-
-Definition compute_incl_lang (l1 l2 : lang) :=
-  if incl_dec (pair_eq_dec string_dec rule_eq_dec) l1 l2 then true else false.
-
-Lemma use_compute_incl_lang (l1 l2 : lang)
-  : compute_incl_lang l1 l2 = true -> incl l1 l2.
-Proof.
-  unfold compute_incl_lang.
-  destruct (incl_dec _ l1 l2); easy.
-Qed.
